fix fizzbuzz

fizzBuzz.fst
@@ -1,33 +1,60 @@
 module FizzBuzz
 
 open LowStar.Printf
+open LowStar.BufferOps
 open FStar.HyperStack.ST
 
+module S = FStar.Seq
 module B = LowStar.Buffer
+module LB = LowStar.Monotonic.Buffer
+module M = LowStar.Modifies
 module U = FStar.UInt
 module U32 = FStar.UInt32
+module ST = FStar.HyperStack.ST
 
-val fizz_buzz: len:U32.t -> Stack C.exit_code
-  (requires fun _ -> true)
-  (ensures fun _ _ _ -> true)
-let fizz_buzz len =
-  let inv h (i: nat) = bool in
-  let body (i: U32.t{ 0 <= U32.v i /\ U32.v i < U32.v len }): Stack unit
-    (requires (fun _ -> true))
+val create_fizzBuzz_array: src:B.buffer string -> n:U32.t -> Stack C.exit_code
+(requires fun h0 -> B.live h0 src /\ B.length src = U32.v n )
+(ensures fun _ _ _ -> true)
+let create_fizzBuzz_array src n =
+  let inv h (i: nat) = B.live h src in
+  let body (i: U32.t{ 0 <= U32.v i /\ U32.v i < U32.v n }): Stack unit
+    (requires (fun h -> inv h (U32.v i)))
     (ensures (fun _ _ _ -> true))
   =
+    let v : string = src.(i) in
     let count: U32.t = U32.(i +^ 1ul) in
+    let fillStr (x:string) = src.(i) <- x in
     let u32Mod (a: U32.t) (b: U32.t{b <> 0ul}) = U32.uint_to_t (U.mod (U32.v a) (U32.v b)) in
-
-    if u32Mod count 15ul = 0ul then printf "%ul: FizzBuzz\n" count done
-    else if u32Mod count 3ul = 0ul then printf "%ul: Fizz\n" count done
-    else if u32Mod count 5ul = 0ul then printf "%ul: Buzz\n" count done
-    else printf "%ul: \n" count done
+      if u32Mod count 15ul = 0ul then (fillStr "FizzBuzz")  
+      else if u32Mod count 3ul = 0ul then (fillStr "Fizz")  
+      else if u32Mod count 5ul = 0ul then (fillStr "Buzz") 
   in
-  C.Loops.for 0ul len inv body;
+  C.Loops.for 0ul n inv body;
+  (* return *) C.EXIT_SUCCESS
+
+val decorate_fizzBuzz_array: src:B.buffer string -> n:U32.t -> Stack C.exit_code
+  (requires fun h0 -> B.live h0 src /\ B.length src = U32.v n )
+  (ensures fun _ _ _ -> true)
+let decorate_fizzBuzz_array src n =
+  let inv h (i: nat) = B.live h src in
+  let body (i: U32.t{ 0 <= U32.v i /\ U32.v i < U32.v n }): Stack unit
+    (requires (fun h -> inv h (U32.v i)))
+    (ensures (fun _ _ _ -> true))
+  =
+    let v : string = src.(i) in
+    let count: U32.t = U32.(i +^ 1ul) in
+    printf "%ul: %s\n" count v done
+  in
+  C.Loops.for 0ul n inv body;
   (* return *) C.EXIT_SUCCESS
 
 let main ()
 =
-  let _ = fizz_buzz 30ul in
+  push_frame ();
+  let n = 10ul in
+  let fillData = "" in
+  let src = B.alloca fillData n in
+  let _ = create_fizzBuzz_array src n in
+  let _ = decorate_fizzBuzz_array src n in
+  pop_frame ();
   C.EXIT_SUCCESS
